lib/Crypto/IsList.lean
@@ -1,5 +1,0 @@
-class IsList (α : Type) where
-  element : Type
-  fromList : List element → α
-
-export IsList (fromList)
