lib/Crypto/OfList.lean
@@ -1,0 +1,11 @@
+
+
+class OfList (α : Type _) (β : outParam (Type _)) (C : outParam (List β → Prop)) where
+  ofList : ∀(l:List β), C l → α
+
+export OfList (ofList)
+
+syntax "#v[" sepBy(term, ", ") "]" : term
+
+macro_rules
+  | `(#v[ $elems,* ]) => `(OfList.ofList [ $elems,* ] (by get_elem_tactic))
